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�� ���� ��� ������ K1 ���� ������� exp(−�xi−xj�2
ε )

�� ��� p = K1 ∗ 1 ����� 1 = (1 1 ... 1)�

�� ����� K2 = K1./(p ∗ p�)

�� ��� v = ����(K2 ∗ 1)

�� ����� K = K2./(v ∗ v�)

�� ����������� K �� [U,S,V] = ���(K)

�� ��� ����������� �� Δ ��� ������������ �� ����� �� K� ��� ���
�������������� φi ��� ������������ �� U(:, i)./U(:, 1)
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��� ��� �� ������ ������� �� ������ 1� ����� Γ ��� �� ��������� ��� ������� ���� ������ ��
������ ��� ���� �������
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����� ��� ������ �� ���� ���� ��� ���������� ���� x �� y �� � ����� ���� t ���� �������
�� ��� ������� ������������ �� ����������� ��� ��� ������ �� ��� ����� ������� x ��� y�
������������� ����� ����� �� ��������� �� � ������ ��� ��� ���� ������ �� � �������� �� ���

�������� ��������� �� � ������������ ��� ������ ������ ������ ��� �� ��������� �� � ������ ��

��� ���� ������� ��� ��� ��� ������� ��� �������������� �� ��� ���������������� �������� ���

����� �� �� ��� ������� ������ ��� ����� ������� ��� ���� ������ ��

pt(α, β) =
1√
4πt

�

j≥0

e−
(α−β+2πj)2

4t =
�

j∈Z
e−j2te2iπj(α−β)

����� α ��� β ��� ��� ����������� ��������� �� ��� ������ �� Γ� ����

pt(α, β) = 1 + 2
�

j≥1

e−j2t(cos(2πjα) cos(2πjβ) + sin(2πjα) sin(2πjβ))
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���� �������� ����� ���� ��� ���� �������� ������ �� t� ���� ��� ���� ����� ����������
�� ���� ���� ��� ��� ���� ��� ��� �� ���������� �������� ����� ��� ��������� α �→
(cos(2πα), sin(2πα))� �� ����� ������ ��� ����� Γ �� ������ ���� � ������ �� ��� ������ ��
��������� ���� ����� ���� ��� ���� ������ ��� �� �������� �� � ������ ������ ����� �� ���
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etD2
t (x, y) =

�

j≥1

e−(j2−1)t
���e2iπjα − e2iπjβ

���
2

=
���e2iπα − e2iπβ

���
2 �

1 + e−3trt(x, y)
�

����� rt(x, y) �� � ������� ���������
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